		\bigbreak

		EXPAND AND PROVE WHY THE INVERSE IS DIFFERENTIABLE AT Y0 

		\bigbreak

		REWORK FINAL PROOF FOR THE INVERSE AT Y0

		\bigbreak

		Examining Caratheodory's characterisation, we have the general form as follows:

		\begin{align*}
		f(x) & = f(x_0) + m_{x_0}(x)(x-x_0)\\
		\end{align*}

		For the inverse function, $f^{-1} (x)$, Charatheodory's characterisation becomes:

		\begin{align*}
		f^{-1} (x) & = f^{-1} (x_0) + m_{x_0}(x)(x-x_0)\\
		\end{align*}

		Replacing $x$ with $y_0$, we arrive at the following result, using the above characterisation of $f^{-1}(x)$.

		\begin{align*}
		f^{-1} (y_0) & = f^{-1} (x_0) + m_{x_0}(y_0)(y_0-x_0)\\
		\therefore f^{-1} (y_0) - f^{-1} (x_0) & = m_{x_0}(y_0)(y_0-x_0)\\
		\therefore \frac{f^{-1} (y_0) - f^{-1} (x_0)}{y_0-x_0} & = m_{x_0}(y_0)\\
		\therefore m_{x_0}(y_0) & = \frac{f^{-1} (y_0) - f^{-1} (x_0)}{y_0-x_0}\\
		\therefore (f^{-1})^\prime(y_0) & = \frac{f^{-1} (y_0) - f^{-1} (x_0)}{y_0-x_0}\\
		& = \frac{1}{\frac{y_0-x_0}{f^{-1} (y_0) - f^{-1} (x_0)}}\\
		& = \frac{1}{\frac{f(f^{-1}(y_0))-f(f^{-1}(x_0))}{f^{-1} (y_0) - f^{-1} (x_0)}} \dots\dots\dots\dots\dots(3)\\
		\end{align*}

		Now consider Caratheodory's characterisation for the function $f(f^{-1}(x))$ at the point $x = y_0$.

		\begin{align*}
		f(x) & = f(x_0) + m_{x_0}(x)(x-x_0)\\
		\therefore f(f^{-1}(x)) & = f(f^{-1}(x_0)) + m_{x_0}(x)(f^{-1}(x)-f^{-1}(x_0))\\
		\therefore f(f^{-1}(y_0)) & = f(f^{-1}(x_0)) + m_{x_0}(y_0)(f^{-1}(y_0)-f^{-1}(x_0))\\
		\therefore f(f^{-1}(y_0)) - f(f^{-1}(x_0)) & = m_{x_0}(y_0)(f^{-1}(y_0)-f^{-1}(x_0))\\
		\therefore \frac{f(f^{-1}(y_0)) - f(f^{-1}(x_0))}{(f^{-1}(y_0)-f^{-1}(x_0))} & = m_{x_0}(y_0)\\
		\therefore m_{x_0}(y_0) & = \frac{f(f^{-1}(y_0)) - f(f^{-1}(x_0))}{(f^{-1}(y_0)-f^{-1}(x_0))}\\
		\therefore f^\prime (f^{-1}(y_0)) & = \frac{f(f^{-1}(y_0)) - f(f^{-1}(x_0))}{(f^{-1}(y_0)-f^{-1}(x_0))} \dots\dots\dots\dots\dots(4)\\
		\end{align*}

		It can now easily be seen that the right hand side of equation $(4)$ is equal to the denominator of equation $(3)$. Thus substituting equation $(4)$ into $(3)$, we get the required result.

		\begin{align*}
		(f^{-1})^\prime(y_0) & = \frac{1}{\frac{f(f^{-1}(y_0))-f(f^{-1}(x_0))}{f^{-1} (y_0) - f^{-1} (x_0)}}\\
		\therefore (f^{-1})^\prime(y_0) & = \frac{1}{f^\prime (f^{-1}(y_0))}\\
		\end{align*}





		%%%
		%
		%
		%
		%
		%
		%%%%
		%%%
		%
		%
		%
		%
		%
		%
		%
		%
		%
		%
		%
		%
		%
		%
		%
		%
		%
		%
		%
		%%
		%
		%
		%
		%
		%%
		%
		%
		%
		%
		%
		%
		%
		%
		%
		%
		%

		
		Let us postulate that the inverse of $f(x)$, $f^{-1}(x)$, at $\displaystyle{y_0 \coloneqq f{x_0}}$, can be written in the form of Caratheodory's characterisation. Thus we have the result:

		\begin{align*}
		f^{-1}(y) & = f^{-1}(y_0) + m_{x_0}(x)(y-y_0)\\
		\end{align*}