		\begin{align*}
		\sqrt{1+x} & \leq 1 + \frac{x}{2}\\
		\sqrt{1+x} - 1 & \leq \frac{x}{2}\\
		\sqrt{1+x} - \sqrt{1} & \leq \frac{x}{2}\\
		\sqrt{1+x} - \sqrt{1+0} & \leq \frac{x}{2}\\
		\frac{\sqrt{1+x} - \sqrt{1+0}}{\frac{x}{2}} & \leq 1\\
		2\left[\frac{\sqrt{1+x} - \sqrt{1+0}}{x}\right] & \leq 1\\
		2\left[\frac{\sqrt{1+x} - \sqrt{1+0}}{x-0}\right] & \leq 1 \dots\dots\dots\dots\dots(1)\\
		\end{align*}

		Now, by the Mean Value Theorem, the expression on the left hand side of the inequality is equal to $f^\prime (x)$, where $f(x) = \sqrt{1+x}$.

		\begin{align*}
		\therefore \frac{\sqrt{1+x} - \sqrt{1+0}}{x-0} & = f^\prime (x)\\
		\therefore 2\left[\frac{\sqrt{1+x} - \sqrt{1+0}}{x-0}\right] & = 2f^\prime (x) \dots\dots\dots\dots\dots(2)\\
		f^\prime (x) & = \frac{1}{2\sqrt{1+x}}\\
		\therefore 2f^\prime (x) & = 2\left[\frac{1}{2\sqrt{1+x}}\right]\\
		& = \frac{1}{\sqrt{1+x}}
		\end{align*}

		\pagebreak

		This expression for $2f^\prime (x)$ is, $\forall x \in (\hspace{0.5mm} -1,\infty \hspace{0.5mm})$, less than 1. Therefore, substituting back into equation $(2)$:

		\begin{align*}
		2\left[\frac{\sqrt{1+x} - \sqrt{1+0}}{x-0}\right] & = 2f^\prime (x)\\
		\therefore 2\left[\frac{\sqrt{1+x} - \sqrt{1+0}}{x-0}\right] & < 1\\
		\end{align*}

		This is the same result as eqaution $(1)$. Thus the inequality $\sqrt{1+x} \leq 1 + \frac{x}{2}$ holds $\forall x \in (\hspace{0.5mm} -1,\infty \hspace{0.5mm})$.