\documentclass[a4paper]{article}

\usepackage{url}
\usepackage{amsmath}
\usepackage{amssymb}
\usepackage{hyperref}

\usepackage{tikz}
\usepackage{graphicx}
\usepackage{enumitem}

\usepackage{titlesec}

\renewcommand{\v}[1]{\textbf{#1}}
\newcommand{\ip}[2]{\langle #1, #2 \rangle}
\newcommand{\e}[1]{\varepsilon_{#1}(u)}
\newcommand{\dote}[1]{\dot{\varepsilon}_{#1}(u)}
\newcommand{\dotg}{\dot{\gamma}(u)}
\newcommand{\ddotg}{\ddot{\gamma}(u)}

\parskip=8pt
\parindent=0pt
\textwidth=6.25in
\oddsidemargin=0pt
\evensidemargin=0pt
\textheight=10in
\topmargin=-0.75in
\baselineskip=11pt

\begin{document}
\pagenumbering{arabic}
\begin{center}
  \vspace{-3mm}
	\textbf{\large {MATH3701 \\
	Higher Topology and Differential Geometry \\
	Assignment}}
\end{center}
\vspace{-5mm}

\begin{enumerate}[leftmargin=\labelsep]
\item[\textbf{1.}]
	Consider $d(l \gamma(u)), u \in I$. Note that $l$ is linear and so $dl = l$.
	\begin{align*}
		d(l \circ \gamma(u)) & = d\gamma(u) \cdot dl(\gamma(u)) \\
		& = d\gamma(u) \cdot l \circ \gamma(u) \hspace{3mm} \text{as $l$ is linear} \\
		& = d\gamma(u) \cdot c.
	\end{align*}
		We know that $\gamma$ sends $u$ into $C$, which is inside the plane $P$. For any $x = \gamma(u)$ inside the plane, by definition, $l \circ \gamma(u) =l(x) = c$. From above, we have $d(l \circ \gamma(u)) = d\gamma(u) \cdot c$. Alternatively, we can differentiate as follows:
	\begin{align*}
		\therefore d(l \circ \gamma(u)) & = d(l(x)) \\
		& = d(c) \\
		& = 0 \\
		\therefore d\gamma(u) \cdot c & = 0 \\
		d\gamma(u) & = 0.
	\end{align*}
		Thus all derivatives of $\gamma$ are zero, so they cannot be linearly independent. Hence $\gamma$ is not Frenet. The curve $\gamma$ lies within a plane, and so it can only curve within a strict range. Given we know $d \gamma(u) = 0$, then the curve is not moving out of this plane and so the derivatives must be scalar multiples, and hence $\gamma$ is not Frenet.
\item[\textbf{2.}]
	\begin{align*}
		\gamma(u) & = (-u,\sin{2u}, \cos{2u})^\mathsf{T} \\
		\dot{\gamma}(u) & = (-1, 2\cos{2u}, -2\sin{2u})^\mathsf{T} \\
		\ddot{\gamma}(u) & = (0, -4\sin{2u}, -4\cos{2u})^\mathsf{T}.
	\end{align*}
	Clearly these are independent and so $\gamma$ is Frenet. For the Frenet Frame we have:
	$$\varepsilon_1(u) = \frac{\dot{\gamma}(u)}{|\dot{\gamma}(u)|} = \frac{1}{\sqrt{5}}(-1, 2\cos{2u}, -2\sin{2u})^\mathsf{T}.$$
	Notice that $\ip{\varepsilon_1(u)}{\ddot{\gamma}(u)} = 0$ and so $\ddot{\gamma}(u)$ is perpendicular to $\varepsilon_1(u)$. Hence for $\varepsilon_2(u)$ we simply normalise $\ddot{\gamma}(u)$.
	$$\varepsilon_2(u) = (0, -\sin{2u}, -\cos{2u})^{\mathsf{T}}.$$
		For $\varepsilon_3(u)$ we take the cross product of the first two vectors in the distinguished Frenet frame.
	\begin{align*}
		\varepsilon_3(u) & = \varepsilon_1(u) \times \varepsilon_2(u) \\
		& = \frac{1}{\sqrt{5}}(-1, 2\cos{2u}, -2\sin{2u})^\mathsf{T} \times (0, -\sin{2u}, -\cos{2u})^{\mathsf{T}} \\
		& = \frac{1}{\sqrt{5}}(-2, -\cos{2u}, \sin{2u})^\mathsf{T}.
	\end{align*}
		Note $\det(\varepsilon_1(u), \varepsilon_2(u), \varepsilon_3(u)) = -1$, we negate $\varepsilon_3(u)$ yielding a determinant of $+1$. Thus the distinguished Frenet frame for $\gamma$ is:
	\begin{align*}
		\varepsilon_1(u) & = \frac{1}{\sqrt{5}}(-1, 2\cos{2u}, -2\sin{2u})^\mathsf{T} \\
		\varepsilon_2(u) & = (0, -\sin{2u}, -\cos{2u})^{\mathsf{T}} \\
		\varepsilon_3(u) &  = \frac{1}{\sqrt{5}}(2, \cos{2u}, -\sin{2u})^\mathsf{T}.
	\end{align*}
\item[\textbf{3.}]
\item[(a)]
	For any $i, j$, we have $\ip{\varepsilon_i(u)}{\varepsilon_j(u)} = 0$ or $1$. In either case we know,
		$$\frac{d}{du}\ip{\varepsilon_i(u)}{\varepsilon_j(u)} = 0.$$
	Using the product rule:
	\begin{align*}
		\ip{\dote{i}}{\e{j}} + \ip{\e{i}}{\dote{j}} & = 0 \\
		\ip{\dote{i}}{\e{j}} & = - \ip{\e{i}}{\dote{j}} \\
		\ip{\dote{i}}{\e{j}} & = - \ip{\dote{j}}{\e{i}} \\
		\therefore w_{ij} & = - w_{ji}.. 
	\end{align*}
\item[(b)]
	Proposition 2 tells us that for $1 \leq i \leq m - 1$, then $Span(\e{1}, ... , \e{i}) = Span(\dot{\gamma}(u), \ddot{\gamma}(u), ... , \gamma^{(i)}(u))$. Clearly $\e{i} \in Span(\e{1}, ... , \e{i}) = Span(\dot{\gamma}(u), \ddot{\gamma}(u), ... , \gamma^{(i)}(u)).$ Hence we can write,
	$$\e{i} = \alpha_1 \dot{\gamma}(u) + \alpha_2 \ddot{\gamma}(u) + ... + \alpha_i \gamma^{(i)}(u).$$
	Differentiating yields:
	\begin{align*}
		\dote{i} & = \alpha_1 \ddot{\gamma}(u) + ... + \alpha_i \gamma^{(i + 1)}(u). \\
		\implies \dote{i} & \in Span(\ddot{\gamma}(u), ... ,\gamma^{(i + 1)}(u)).
	\end{align*}
		Note that $Span(\ddot{\gamma}(u), ... ,\gamma^{(i + 1)}(u))$ is a subset of $Span(\dot{\gamma}(u), \ddot{\gamma}(u), ..., \gamma^{(i + 1)}(u)) = Span(\e{1}, ... , \e{i + 1}).$
		$$\therefore \dote{i+1} \in Span(\dot{\gamma}(u), \ddot{\gamma}(u), ..., \gamma^{(i + 1)}(u)).$$
\item[(c)]
	First note that given $\dote{i} \in Span(\e{1}, \e{2}, ... , \e{i + 1})$ then we can write.
	\begin{align*}
		\dote{i} & = \alpha_1 \e{1} + \alpha_2 \e{2} + ... + \alpha_{i + 1} \e{i + 1}. \\
		\implies w_{ij} & = \ip{\dote{i}}{\e{j}} \\
		& = \ip{\alpha_1 \e{1} + \alpha_2 \e{2} + ... + \alpha_{i + 1} \e{i + 1}}{\e{j}} \\
		& = \begin{cases}
			0 & j > i + 1 \\
			\alpha_j & j \leq i + 1.
		\end{cases}
	\end{align*}
	We can obtain a similar expression for $w_{ji}$,
	$$w_{ji} = \begin{cases}
			0 & i > j + 1 \\
			\beta_i & i \leq j + 1.
		\end{cases}$$
	We also know that $w_{ij} = -w_{ji}$. Hence we have the following cases: \\ [1mm]
	\textit{(1) $i > j + 1$ or $j > i + 1$:} \\ [1mm]
		In this case either $w_{ij} = 0$ or $w_{ji} = 0$. Either way, as $w_{ij} = -w_{ji}$, we know that $w_{ij} = 0$. \\ [1mm]
	\textit{(2) $i \leq j + 1$ and $j \leq i + 1$, this is equivalent to saying $|i - j| = 1$:} \\ [1mm]
	$w_{ij} = \alpha_j$ and $w_{ji} = \beta_i$. Hence we also have the relationship $\alpha_j = -\beta_i$. \\ [1.5mm]
	Thus $w_{ij} = 0$ unless $|i - j| = 1$.

\item[\textbf{4.}]
	Note we have the following distinguished Frenet frame for $\gamma$.
	\begin{align*}
		\varepsilon_1(u) & = \frac{1}{\sqrt{5}}(-1, 2\cos{2u}, -2\sin{2u})^\mathsf{T} \\
		\varepsilon_2(u) & = (0, -\sin{2u}, -\cos{2u})^{\mathsf{T}} \\
		\varepsilon_3(u) &  = \frac{1}{\sqrt{5}}(2, \cos{2u}, -\sin{2u})^\mathsf{T}.
	\end{align*}
	Computing $\kappa_1(u)$ and $\kappa_2(u)$:
	\begin{align*}
		\kappa_1(u) & = \frac{\ip{\dote{1}}{\e{2}}}{|\dotg|} \\
		& = \frac{\ip{\frac{1}{\sqrt{5}} (0, -4\sin{2u}, -4\cos{2u})^{\mathsf{T}}}{(0, -\sin{2u}, -\cos{2u})^{\mathsf{T}}}}{\sqrt{5}} \\
		\therefore \kappa_1(u) & = \frac{4}{5}. \\
		\kappa_2(u) & = \frac{\ip{\dote{2}}{\e{3}}}{|\dotg|} \\
		& = \frac{\ip{(0, -2\cos{2u}, 2\sin{2u})^{\mathsf{T}}}{\frac{1}{\sqrt{5}} (2, \cos{2u}, -\sin{2u})^{\mathsf{T}}}}{\sqrt{5}} \\
		\therefore \kappa_2(u) & = -\frac{2}{5}.
	\end{align*}

\item[\textbf{5.}]
	Given a unit speed Frenet curve $\gamma : I \rightarrow \mathbb{R}^m$, we know that $|\dotg| = 1$ and, $$C(u) = (\dotg, \ddotg, ... , \gamma^{(m)}(u)).$$
	We can also express each column $\gamma^{(i)}(u)$ as a linear combination of the first $i$ vectors in the Frenet frame. 
	$$\gamma^{(i)}(u) = \alpha_1 \e{1} + \alpha_2 \e{2} + ... + \alpha_i \e{i}.$$

\end{enumerate}
\end{document}
